Prefix: : <http://example.org/pumpwithfirmware/>
Prefix: acme: <http://example.org/>
Prefix: dc: <http://purl.org/dc/elements/1.1/>
Prefix: dcterms: <http://purl.org/dc/terms/>
Prefix: iof-av: <https://spec.industrialontologies.org/ontology/core/meta/AnnotationVocabulary/>
Prefix: lis: <http://rds.posccaesar.org/ontology/lis14/rdl/>
Prefix: owl: <http://www.w3.org/2002/07/owl#>
Prefix: plm: <http://rds.posccaesar.org/ontology/plm/rdl/>
Prefix: rdf: <http://www.w3.org/1999/02/22-rdf-syntax-ns#>
Prefix: rdfs: <http://www.w3.org/2000/01/rdf-schema#>
Prefix: sosa: <http://www.w3.org/ns/sosa/>
Prefix: td: <https://www.w3.org/2019/wot/td>
Prefix: xml: <http://www.w3.org/XML/1998/namespace>
Prefix: xsd: <http://www.w3.org/2001/XMLSchema#>



Ontology: <http://example.org/pumpwithfirmware>
<http://example.org/pumpwithfirmware/0.0.3>
Import: <http://rds.posccaesar.org/ontology/lis14/ont/core/1.1-alpha.0>

Annotations: 
    dcterms:contributor "Johan W. Kl√ºwer, DNV",
    dcterms:contributor "Maja Milicic Brandt, Siemens",
    dcterms:contributor "Melinda Hodkiewicz, UWA",
    dcterms:contributor "Mikkel Haggren Brynildsen, Grundfos"

AnnotationProperty: <http://www.w3.org/2004/02/skos/core#note>

    
AnnotationProperty: dcterms:contributor

    
AnnotationProperty: dcterms:description

    
AnnotationProperty: iof-av:naturalLanguageDefinition

    
AnnotationProperty: iof-av:usageNote

    
AnnotationProperty: owl:deprecated

    
AnnotationProperty: rdfs:comment

    
AnnotationProperty: rdfs:label

    
AnnotationProperty: rdfs:seeAlso

    
Datatype: rdf:PlainLiteral

    
Datatype: xsd:boolean

    
Datatype: xsd:decimal

    
Datatype: xsd:integer

    
Datatype: xsd:string

    
ObjectProperty: acme:hasInput

    SubPropertyOf: 
        lis:hasPassiveParticipant
    
    
ObjectProperty: lis:concretizedBy

    
ObjectProperty: lis:concretizes

    
ObjectProperty: lis:connectedTo

    
ObjectProperty: lis:contains

    
ObjectProperty: lis:creates

    
ObjectProperty: lis:datumUOM

    
ObjectProperty: lis:hasActiveParticipant

    
ObjectProperty: lis:hasFunction

    
ObjectProperty: lis:hasFunctionalPart

    
ObjectProperty: lis:hasPart

    
ObjectProperty: lis:hasParticipant

    
ObjectProperty: lis:hasPassiveParticipant

    
ObjectProperty: lis:hasPhysicalQuantity

    
ObjectProperty: lis:hasQuality

    
ObjectProperty: lis:partOf

    
ObjectProperty: lis:participantIn

    
ObjectProperty: lis:profileOfQuality

    
ObjectProperty: lis:profileQuantityDatum

    
ObjectProperty: lis:qualityOf

    
ObjectProperty: lis:qualityQuantifiedAs

    
ObjectProperty: lis:realizes

    
ObjectProperty: lis:representedIn

    
ObjectProperty: lis:residesIn

    
ObjectProperty: sosa:hasResult

    Annotations: 
        rdfs:label "hasResult",
        rdfs:seeAlso <http://www.w3.org/ns/sosa/hasResult>,
        iof-av:naturalLanguageDefinition "Relation linking an observation activity and a sensor and  a result. The range should only be one observation."
    
    SubPropertyOf: 
        lis:creates
    
    
ObjectProperty: sosa:madeBySensor

    SubPropertyOf: 
        lis:hasActiveParticipant
    
    
ObjectProperty: sosa:observedProperty

    Annotations: 
        rdfs:label "observedProperty",
        rdfs:seeAlso <http://www.w3.org/ns/sosa/observedProperty>,
        iof-av:naturalLanguageDefinition "Relation linking an observation activity profile to the quality of interest that was observed."
    
    SubPropertyOf: 
        lis:profileOfQuality
    
    
DataProperty: acme:WoTDataProperties

    SubPropertyOf: 
        owl:topDataProperty
    
    
DataProperty: acme:hasDeveloper

    
DataProperty: acme:hasFormHref

    
DataProperty: acme:hasResolutionInBits

    Domain: 
        lis:InformationObject
    
    SubPropertyOf: 
        owl:topDataProperty
    
    
DataProperty: acme:hasSignificantDigits

    
DataProperty: acme:hasVersion

    
DataProperty: acme:majorVersion

    SubPropertyOf: 
        acme:hasVersion
    
    
DataProperty: acme:minorVersion

    SubPropertyOf: 
        acme:hasVersion
    
    
DataProperty: acme:multipleOf

    SubPropertyOf: 
        acme:WoTDataProperties
    
    
DataProperty: acme:patchVersion

    SubPropertyOf: 
        acme:hasVersion
    
    
DataProperty: lis:datumValue

    
DataProperty: owl:topDataProperty

    
Class: acme:CalibrationDatum

    SubClassOf: 
        lis:ScalarQuantityDatum
    
    
Class: acme:CalibrationMax

    SubClassOf: 
        acme:CalibrationDatum
    
    
Class: acme:CalibrationMin

    SubClassOf: 
        acme:CalibrationDatum
    
    
Class: acme:CoolingPump

    SubClassOf: 
        acme:Pump
    
    
Class: acme:DataStream

    SubClassOf: 
        lis:PhysicalArtefact
    
    
Class: acme:DigitallyExposeLiquidTemperature

    SubClassOf: 
        acme:DigitallyExposeState
    
    
Class: acme:DigitallyExposeState

    Annotations: 
        rdfs:seeAlso <https://www.w3.org/2019/wot/tdPropertyAffordance>
    
    SubClassOf: 
        lis:Function
    
    
Class: acme:E-78-130-F-M-270

    SubClassOf: 
        acme:CoolingPump
    
    
Class: acme:ElectronicsController

    Annotations: 
        rdfs:label "ElectronicsController"
    
    SubClassOf: 
        lis:PhysicalArtefact
    
    
Class: acme:EstimatedDatum

    SubClassOf: 
        lis:QualityDatum
    
    
Class: acme:HandleIOTCall

    SubClassOf: 
        acme:SoftwareProcess
    
    
Class: acme:InstalledSoftware

    SubClassOf: 
        lis:PhysicalArtefact
    
    
Class: acme:Pump

    SubClassOf: 
        lis:PhysicalArtefact
    
    
Class: acme:PumpHousing

    Annotations: 
        rdfs:label "PumpHousing",
        iof-av:naturalLanguageDefinition "Physical artefact that encloses, and contains the moving parts of the hydraulics. Gives direction to the flow of the pumped liquid."
    
    SubClassOf: 
        lis:PhysicalArtefact
    
    
Class: acme:PumpTemperatureSensor

    Annotations: 
        rdfs:label "PumpTemperatureSensor",
        iof-av:naturalLanguageDefinition "A physical artefact that measures a physical quantity and converts it into a digital representation which can be read by a connected equipment."
    
    SubClassOf: 
        lis:PhysicalArtefact,
        lis:connectedTo some acme:PumpHousing
    
    
Class: acme:QualityDatum_2SD

    SubClassOf: 
        lis:QualityDatum,
        acme:hasSignificantDigits only xsd:integer[>= 2]
    
    
Class: acme:SensingActivity

    SubClassOf: 
        lis:Activity
    
    
Class: acme:SoftwareAgent

    SubClassOf: 
        lis:PhysicalArtefact
    
    
Class: acme:SoftwareAgentFunction

    SubClassOf: 
        lis:Function
    
    
Class: acme:SoftwareProcess

    SubClassOf: 
        lis:Activity
    
    
Class: acme:Temperature

    Annotations: 
        rdfs:label "Temperature",
        rdfs:seeAlso <http://rds.posccaesar.org/ontology/plm/rdl/PCA_100003601>,
        rdfs:seeAlso "ISO 80000-5:2019 5.1 \"thermodynamic temperature\"",
        iof-av:naturalLanguageDefinition "Partial derivative of internal energy with respect to entropy at constant volume and constant number of particles in the system. 

Differences in thermodynamic temperatures may be expressed in for instance Kelvin or degrees Celcius."
    
    SubClassOf: 
        lis:PhysicalQuantity
    
    
Class: acme:TemperatureSensingActivity

    SubClassOf: 
        acme:SensingActivity
    
    
Class: lis:Activity

    
Class: lis:ActivityProfile

    
Class: lis:Function

    
Class: lis:InformationObject

    
Class: lis:Person

    
Class: lis:PhysicalArtefact

    
Class: lis:PhysicalObject

    
Class: lis:PhysicalQuantity

    
Class: lis:Quality

    
Class: lis:QualityDatum

    
Class: lis:ScalarQuantityDatum

    
Class: lis:Scale

    
Class: lis:SoftwareArtefact

    
Class: lis:Stream

    
Individual: <http://example.org/5000.02.01.PU001.Pump>

    Annotations: 
        dcterms:description "5000.01.01.PU001 identifies Pump 001, in plant subsection 01, in plant section 02 at Plant 5000."
    
    Types: 
        acme:E-78-130-F-M-270
    
    Facts:  
     lis:contains  acme:PU001.PumpedFluid,
     lis:hasFunctionalPart  acme:CT001.Controller,
     lis:hasFunctionalPart  acme:PU001.Housing,
     lis:hasFunctionalPart  acme:TT101.TempSensor
    
    
Individual: acme:CT001.ControlScheduler.Firmware

    Annotations: 
        dcterms:description "The Firmware (a software artefact) compiled by Grundfos containing instructions for operating the Controller"
    
    Types: 
        lis:SoftwareArtefact
    
    
Individual: acme:CT001.ControlScheduler.Function

    Annotations: 
        dcterms:description "The software agent function required/performed by the ControlScheduler.InstalledFirmware"
    
    Types: 
        acme:SoftwareAgentFunction
    
    
Individual: acme:CT001.ControlScheduler.InstalledFirmware

    Annotations: 
        dcterms:description "The as-installed version of ControlScheduler.Firmware on the CT001 controller. This InstalledFirmware  participates in the TT101.TempSensingActivity"
    
    Types: 
        acme:InstalledSoftware
    
    Facts:  
     lis:concretizes  acme:CT001.ControlScheduler.Firmware,
     lis:hasFunction  acme:CT001.ControlScheduler.Function,
     lis:participantIn  acme:TT101.TempSensingActivity
    
    
Individual: acme:CT001.ControlSoftware_v1.1.1

    Annotations: 
        dcterms:description "Software installed on the pump controller CT001 to manage communication between the transmitter TT001, store the data and manage the IOT calls"
    
    Types: 
        lis:SoftwareArtefact
    
    
Individual: acme:CT001.Controller

    Annotations: 
        dcterms:description "CT001 is the controller for Pump PU001 purchased from Siemens by Grundfos"
    
    Types: 
        acme:ElectronicsController
    
    Facts:  
     lis:hasFunctionalPart  acme:CT001.ControlScheduler.InstalledFirmware,
     lis:hasFunctionalPart  acme:CT001.TempMonitoringInstalledFirmware
    
    
Individual: acme:CT001.FunctionToDigitallyExposeTemp

    Annotations: 
        dcterms:description "Function of the CT001 TempMonitoringInstalledFirmware to digitally expose (sample/capture) the temperature on the TT101 sensor"
    
    Types: 
        acme:DigitallyExposeLiquidTemperature
    
    
Individual: acme:CT001.HandleTempIoTCallAndTempEstimation

    Annotations: 
        dcterms:description "A function specifically for handling the IOT call and estimation steps for the temperature data"
    
    Types: 
        lis:Function
    
    
Individual: acme:CT001.HandleTempIoTCallAndTempEstimation.Firmware

    Annotations: 
        dcterms:description "The firmware (compiled by Grundfos) that performs the functions required for the IOT call and temperature estimation. This firmware has different versions as updates to the code are made e.g. minor version 2, patch version 4 and major version 10."
    
    Types: 
        lis:SoftwareArtefact
    
    Facts:  
     acme:majorVersion  10,
     acme:minorVersion  2,
     acme:patchVersion  4
    
    
Individual: acme:CT001.HandleTempIoTCallAndTempEstimation.InstalledFirmware

    Annotations: 
        dcterms:description "The as-installed version of HandleTempIoTCallAndTempEstimationr.Firmware on the CT001 controller. This InstalledFirmware  participates in the CT001.IoTServerProcess001 activity"
    
    Types: 
        acme:InstalledSoftware
    
    Facts:  
     lis:concretizes  acme:CT001.HandleTempIoTCallAndTempEstimation.Firmware,
     lis:hasFunction  acme:CT001.HandleTempIoTCallAndTempEstimation,
     lis:participantIn  acme:CT001.IoTServerProcess001
    
    
Individual: acme:CT001.IoTServerProcess001

    Annotations: 
        dcterms:description "This process takes as input the temperature reading from TT101.tempReading002 and IoT call message protocols to produce a time-stamped value for the PU001 fluid temperature estimation in an appropriate format. It delivers the this datum to the right output port adhering to the WoT communication protocol."
    
    Types: 
        acme:HandleIOTCall
    
    Facts:  
     acme:hasInput  acme:TT101.tempReading002,
     lis:hasPassiveParticipant  acme:CT101.IoT.Message,
     lis:realizes  acme:CT001.HandleTempIoTCallAndTempEstimation,
     sosa:hasResult  acme:PU001.fluidTempEst_TimeStampedIndex54678
    
    
Individual: acme:CT001.TempMonitoringInstalledFirmware

    Annotations: 
        dcterms:description "The as-installed version of CT001.ControlSoftware on the CT001 controller. This InstalledFirmware  participates in the CT001.IoTServerProcess"
    
    Types: 
        acme:InstalledSoftware
    
    Facts:  
     lis:concretizes  acme:CT001.ControlSoftware_v1.1.1,
     lis:hasFunction  acme:CT001.FunctionToDigitallyExposeTemp,
     lis:participantIn  acme:CT001.IoTServerProcess001
    
    
Individual: acme:CT001.temp.Result

    Annotations: 
        dcterms:description "The value of the actual temperature of the pump housing stored in the CT001 controller. This value is what is measured by temperature transmitter embedded in the PU001 pump housing."
    
    Types: 
        acme:QualityDatum_2SD
    
    
Individual: acme:CT101.IoT.Message

    Annotations: 
        dcterms:description "A DataStream for the PU001.fluidTempEst_TimeStampedIndex54678 message transmitted using the Iot protocol"
    
    Types: 
        acme:DataStream
    
    Facts:  
     lis:concretizes  acme:PU001.fluidTempEst_TimeStampedIndex54678
    
    
Individual: acme:Celsius

    Annotations: 
        dcterms:description "a unit of measure for temperature"
    
    Types: 
        lis:Scale
    
    
Individual: acme:PU001.FluidTemperature

    Annotations: 
        dcterms:description "The actual (but not directly measured) temperature of the fluid inside PU001. The temperature transmitter is located inside the pump housing but does not have direct contact with the pumped fluid. The reading made by the sensor will have some measurement error and depend the placement of the sensor and the thermal characteristics of the housing."
    
    Types: 
        acme:Temperature
    
    Facts:  
     lis:qualityQuantifiedAs  acme:PU001.fluidTempEst_TimeStampedIndex54678
    
    
Individual: acme:PU001.Housing

    Annotations: 
        dcterms:description "The housing of the pump PU001"
    
    Types: 
        acme:PumpHousing
    
    Facts:  
     lis:contains  acme:PU001.PumpedFluid,
     lis:hasPhysicalQuantity  acme:PU001.HousingTemperature
    
    
Individual: acme:PU001.HousingTemperature

    Annotations: 
        dcterms:description "The actual temperature of the pump housing, as measured by the temperature transmitter which is installed in a hole drilled in the pump housing. This is not the same as the pumped fluid temperature as the fluid temperature cannot be directly measured, see PU001.FluidTemperature for more information."
    
    Types: 
        acme:Temperature
    
    Facts:  
     lis:qualityQuantifiedAs  acme:CT001.temp.Result
    
    
Individual: acme:PU001.PumpedFluid

    Annotations: 
        dcterms:description "The fluid that is being pumped by the pump, it is contained by the pump housing."
    
    Types: 
        lis:Stream
    
    Facts:  
     lis:hasPhysicalQuantity  acme:PU001.FluidTemperature
    
    
Individual: acme:PU001.fluidTempEst_TimeStampedIndex54678

    Annotations: 
        dcterms:description "This is a time stamped value for the temperature of the fluid read in the Cloud of ACME Digital Dairy and ACME. It is the value-delivery step for both business units. All prior steps in this ontology are intended to ensure the measurement precision of the data reported in this time stamped value. It has the data property for the required precision of the temperature reading."
    
    Types: 
        acme:EstimatedDatum
    
    Facts:  
     acme:multipleOf  0.1
    
    
Individual: acme:PU001.fluidTempStoredInUsersCloud_54678

    Annotations: 
        dcterms:description "This is the part in the code, installed in the User's cloud software, that holds the time stamped value for the temperature of the fluid in the pump."
    
    Types: 
        acme:InstalledSoftware
    
    Facts:  
     lis:concretizes  acme:PU001.fluidTempEst_TimeStampedIndex54678
    
    
Individual: acme:TT101.DownSamplingActivity

    Annotations: 
        dcterms:description "The process of downsampling from 16-bit to 8-bit, this process takes as input TT101.tempReading001 and outputs TT101.tempReading002. It is this part of the process that the ontology is designed to track as the downsampling process results in a change in precision of the reported pump fluid temperature value."
    
    Types: 
        lis:Activity
    
    Facts:  
     acme:hasInput  acme:TT101.tempReading001,
     sosa:hasResult  acme:TT101.tempReading002
    
    
Individual: acme:TT101.Temp.Observation

    Annotations: 
        dcterms:description "The activity (involving the temperature transmitter sensor TT101 installed in the pump housing) of observing the temperature."
    
    Types: 
        lis:ActivityProfile
    
    Facts:  
     lis:partOf  acme:TT101.TempSensingActivity,
     lis:profileQuantityDatum  acme:TT101.tempReading001,
     sosa:madeBySensor  acme:TT101.TempSensor,
     sosa:observedProperty  acme:PU001.HousingTemperature
    
    
Individual: acme:TT101.TempSensingActivity

    Annotations: 
        dcterms:description "Process controlled by the CT001.ControlScheduler.InstalledFirmware which has part the 16 bit to 8 bit downsampling activity described in TT101.DownSamplingActivity."
    
    Types: 
        acme:TemperatureSensingActivity
    
    Facts:  
     lis:hasPart  acme:TT101.DownSamplingActivity,
     lis:realizes  acme:CT001.ControlScheduler.Function
    
    
Individual: acme:TT101.TempSensor

    Annotations: 
        rdfs:comment "Temperature sensor and its associated electronics (firmware) embedded in the pump housing."
    
    Types: 
        acme:PumpTemperatureSensor
    
    Facts:  
     lis:connectedTo  acme:PU001.Housing,
     lis:hasFunctionalPart  acme:TT101.TempSensor.InstalledFirmware,
     lis:hasQuality  acme:TT101.TempSensorCalibration
    
    
Individual: acme:TT101.TempSensor.InstalledFirmware

    Annotations: 
        dcterms:description "The version of firmware installed in PU001.TempSensor.TT101"
    
    Types: 
        acme:InstalledSoftware
    
    Facts:  
     lis:participantIn  acme:TT101.TempSensingActivity
    
    
Individual: acme:TT101.TempSensorCalibration

    Annotations: 
        dcterms:description "Holds the calibration parameters for the TT101.TempSensorCalibration. In this use case two example parameters are provided, calibration max and a calibration min."
    
    Types: 
        lis:Quality
    
    Facts:  
     lis:qualityQuantifiedAs  acme:TT101.TempSensorCalibrationMax,
     lis:qualityQuantifiedAs  acme:TT101.TempSensorCalibrationMin
    
    
Individual: acme:TT101.TempSensorCalibrationMax

    Annotations: 
        dcterms:description "Contains the data values for calibration and the units (celsius). In this example, there are two parameters, calibration max and calibration min. These describe the expected range of the temperature readings for this pump installation."
    
    Types: 
        acme:CalibrationMax
    
    Facts:  
     lis:datumUOM  acme:Celsius,
     lis:datumValue  95
    
    
Individual: acme:TT101.TempSensorCalibrationMin

    Annotations: 
        dcterms:description "Contains the data values for calibration and the units (celsius). In this example, there are two parameters, calibration max and calibration min. These describe the expected range of the temperature readings for this pump installation."
    
    Types: 
        acme:CalibrationMin
    
    Facts:  
     lis:datumUOM  acme:Celsius,
     lis:datumValue  0
    
    
Individual: acme:TT101.tempReading001

    Annotations: 
        dcterms:description "TT101.tempReading001 holds the 16 bit resolution value of the temperature reading and is the input to the TT101.DownSamplingActivity"
    
    Types: 
        lis:QualityDatum
    
    Facts:  
     acme:hasResolutionInBits  16
    
    
Individual: acme:TT101.tempReading002

    Annotations: 
        dcterms:description "TT101.tempReading002 holds the 8 bit resolution value of the temperature reading and is the output of the TT101.DownSamplingActivity"
    
    Types: 
        lis:QualityDatum
    
    Facts:  
     acme:hasResolutionInBits  8
    
    
Individual: acme:WotThingDescriptionLiquidTemperature-ThingDescription

    Annotations: 
        dcterms:description "Contains the precision for the temperature estimation (1 deg C in this example) in the WoT protocol format."
    
    Types: 
        lis:InformationObject
    
    Facts:  
     lis:concretizedBy  acme:CT001.IoTServerProcess001,
     acme:hasFormHref  "1/40000?quantity=1"
    
    
