Prefix: : <http://example.org/pumpwithfirmware/0.0.1>
Prefix: acme: <http://example.org/>
Prefix: dc: <http://purl.org/dc/elements/1.1/>
Prefix: dcterms: <http://purl.org/dc/terms/>
Prefix: iof-av: <https://spec.industrialontologies.org/ontology/core/meta/AnnotationVocabulary/>
Prefix: lis: <http://rds.posccaesar.org/ontology/lis14/rdl/>
Prefix: owl: <http://www.w3.org/2002/07/owl#>
Prefix: plm: <http://rds.posccaesar.org/ontology/plm/rdl/>
Prefix: rdf: <http://www.w3.org/1999/02/22-rdf-syntax-ns#>
Prefix: rdfs: <http://www.w3.org/2000/01/rdf-schema#>
Prefix: sosa: <http://www.w3.org/ns/sosa/>
Prefix: td: <https://www.w3.org/2019/wot/td>
Prefix: xml: <http://www.w3.org/XML/1998/namespace>
Prefix: xsd: <http://www.w3.org/2001/XMLSchema#>



Ontology: <http://example.org/pumpwithfirmware>
<http://example.org/pumpwithfirmware/0.0.2>
Import: <http://rds.posccaesar.org/ontology/lis14/ont/core/1.1-alpha.0>

Annotations: 
    dcterms:contributor "Johan W. Kl√ºwer, DNV",
    dcterms:contributor "Maja Milicic Brandt, Siemens",
    dcterms:contributor "Melinda Hodkiewicz, UWA",
    dcterms:contributor "Mikkel Haggren Brynildsen, Grundfos"

AnnotationProperty: <http://www.w3.org/2004/02/skos/core#note>

    
AnnotationProperty: acme:visibleInDiagram

    Annotations: 
        rdfs:comment "",
        iof-av:usageNote "an auxiliary notation to be able to control the automatic generation of visuals of the knowledge graph."
    
    SubPropertyOf: 
        <http://www.w3.org/2004/02/skos/core#note>
    
    
AnnotationProperty: dcterms:contributor

    
AnnotationProperty: dcterms:description

    
AnnotationProperty: iof-av:naturalLanguageDefinition

    
AnnotationProperty: iof-av:usageNote

    
AnnotationProperty: owl:deprecated

    
AnnotationProperty: rdfs:comment

    
AnnotationProperty: rdfs:label

    
AnnotationProperty: rdfs:seeAlso

    
Datatype: rdf:PlainLiteral

    
Datatype: xsd:boolean

    
Datatype: xsd:decimal

    
Datatype: xsd:integer

    
Datatype: xsd:string

    
ObjectProperty: acme:hasInput

    SubPropertyOf: 
        lis:hasPassiveParticipant
    
    
ObjectProperty: lis:concretizedBy

    
ObjectProperty: lis:concretizes

    
ObjectProperty: lis:connectedTo

    
ObjectProperty: lis:contains

    
ObjectProperty: lis:creates

    
ObjectProperty: lis:datumUOM

    
ObjectProperty: lis:hasActiveParticipant

    
ObjectProperty: lis:hasFunction

    
ObjectProperty: lis:hasFunctionalPart

    
ObjectProperty: lis:hasPart

    
ObjectProperty: lis:hasParticipant

    
ObjectProperty: lis:hasPassiveParticipant

    
ObjectProperty: lis:hasPhysicalQuantity

    
ObjectProperty: lis:hasQuality

    
ObjectProperty: lis:partOf

    
ObjectProperty: lis:participantIn

    
ObjectProperty: lis:profileOfQuality

    
ObjectProperty: lis:profileQuantityDatum

    
ObjectProperty: lis:qualityOf

    
ObjectProperty: lis:qualityQuantifiedAs

    
ObjectProperty: lis:realizes

    
ObjectProperty: lis:representedIn

    
ObjectProperty: lis:residesIn

    
ObjectProperty: sosa:hasResult

    Annotations: 
        rdfs:label "hasResult",
        rdfs:seeAlso <http://www.w3.org/ns/sosa/hasResult>,
        iof-av:naturalLanguageDefinition "Relation linking an observation activity and a sensor and  a result. The range should only be one observation."
    
    SubPropertyOf: 
        lis:creates
    
    
ObjectProperty: sosa:madeBySensor

    SubPropertyOf: 
        lis:hasActiveParticipant
    
    
ObjectProperty: sosa:observedProperty

    Annotations: 
        rdfs:label "observedProperty",
        rdfs:seeAlso <http://www.w3.org/ns/sosa/observedProperty>,
        iof-av:naturalLanguageDefinition "Relation linking an observation activity profile to the quality of interest that was observed."
    
    SubPropertyOf: 
        lis:profileOfQuality
    
    
DataProperty: acme:WoTDataProperties

    SubPropertyOf: 
        owl:topDataProperty
    
    
DataProperty: acme:hasDeveloper

    
DataProperty: acme:hasFormHref

    
DataProperty: acme:hasResolutionInBits

    Domain: 
        lis:InformationObject
    
    SubPropertyOf: 
        owl:topDataProperty
    
    
DataProperty: acme:hasSignificantDigits

    
DataProperty: acme:hasVersion

    
DataProperty: acme:majorVersion

    SubPropertyOf: 
        acme:hasVersion
    
    
DataProperty: acme:minorVersion

    SubPropertyOf: 
        acme:hasVersion
    
    
DataProperty: acme:multipleOf

    SubPropertyOf: 
        acme:WoTDataProperties
    
    
DataProperty: acme:patchVersion

    SubPropertyOf: 
        acme:hasVersion
    
    
DataProperty: lis:datumValue

    
DataProperty: owl:topDataProperty

    
Class: acme:CalibrationDatum

    SubClassOf: 
        lis:ScalarQuantityDatum
    
    
Class: acme:CalibrationMax

    SubClassOf: 
        acme:CalibrationDatum
    
    
Class: acme:CalibrationMin

    SubClassOf: 
        acme:CalibrationDatum
    
    
Class: acme:CoolingPump

    Annotations: 
        acme:visibleInDiagram "M2"
    
    SubClassOf: 
        acme:Pump
    
    
Class: acme:DataStream

    SubClassOf: 
        lis:PhysicalArtefact
    
    
Class: acme:DigitallyExposeLiquidTemperature

    SubClassOf: 
        acme:functionToDigitallyExposeState
    
    
Class: acme:E-78-130-F-M-270

    Annotations: 
        acme:visibleInDiagram "M2",
        acme:visibleInDiagram "M3"
    
    SubClassOf: 
        acme:CoolingPump
    
    
Class: acme:ElectronicsController

    Annotations: 
        acme:visibleInDiagram "M3",
        rdfs:label "ElectronicsController"
    
    SubClassOf: 
        lis:PhysicalArtefact
    
    
Class: acme:EstimatedDatum

    SubClassOf: 
        lis:QualityDatum
    
    
Class: acme:Firmware

    Annotations: 
        acme:visibleInDiagram "M8"
    
    SubClassOf: 
        lis:Quality
    
    
Class: acme:HandleIOTCall

    SubClassOf: 
        acme:SoftwareProcess
    
    
Class: acme:InstalledSoftware

    SubClassOf: 
        lis:PhysicalArtefact
    
    
Class: acme:Pump

    Annotations: 
        acme:visibleInDiagram "M2"
    
    SubClassOf: 
        lis:PhysicalArtefact
    
    
Class: acme:PumpHousing

    Annotations: 
        acme:visibleInDiagram "M3",
        rdfs:label "PumpHousing",
        iof-av:naturalLanguageDefinition "Physical artefact that encloses, and contains the moving parts of the hydraulics. Gives direction to the flow of the pumped liquid."
    
    SubClassOf: 
        lis:PhysicalArtefact
    
    
Class: acme:PumpTemperatureSensor

    Annotations: 
        acme:visibleInDiagram "M3",
        rdfs:label "PumpTemperatureSensor",
        iof-av:naturalLanguageDefinition "A physical artefact that measures a physical quantity and converts it into a digital representation which can be read by a connected equipment."
    
    SubClassOf: 
        lis:PhysicalArtefact,
        lis:connectedTo some acme:PumpHousing
    
    
Class: acme:QualityDatum_2SD

    SubClassOf: 
        lis:QualityDatum,
        acme:hasSignificantDigits only xsd:integer[>= 2]
    
    
Class: acme:SensingActivity

    SubClassOf: 
        lis:Activity
    
    
Class: acme:SoftwareAgent

    SubClassOf: 
        lis:PhysicalArtefact
    
    
Class: acme:SoftwareAgentFunction

    SubClassOf: 
        lis:Function
    
    
Class: acme:SoftwareProcess

    SubClassOf: 
        lis:Activity
    
    
Class: acme:Temperature

    Annotations: 
        rdfs:label "Temperature",
        rdfs:seeAlso <http://rds.posccaesar.org/ontology/plm/rdl/PCA_100003601>,
        rdfs:seeAlso "ISO 80000-5:2019 5.1 \"thermodynamic temperature\"",
        iof-av:naturalLanguageDefinition "Partial derivative of internal energy with respect to entropy at constant volume and constant number of particles in the system. 

Differences in thermodynamic temperatures may be expressed in for instance Kelvin or degrees Celcius."
    
    SubClassOf: 
        lis:PhysicalQuantity
    
    
Class: acme:TemperatureSensingActivity

    SubClassOf: 
        acme:SensingActivity
    
    
Class: acme:functionToDigitallyExposeState

    Annotations: 
        rdfs:seeAlso <https://www.w3.org/2019/wot/tdPropertyAffordance>
    
    SubClassOf: 
        lis:Function
    
    
Class: lis:Activity

    
Class: lis:ActivityProfile

    
Class: lis:Function

    
Class: lis:InformationObject

    
Class: lis:Person

    
Class: lis:PhysicalArtefact

    Annotations: 
        acme:visibleInDiagram "M2"
    
    
Class: lis:PhysicalObject

    
Class: lis:PhysicalQuantity

    
Class: lis:Quality

    
Class: lis:QualityDatum

    
Class: lis:ScalarQuantityDatum

    
Class: lis:Scale

    
Class: lis:SoftwareArtefact

    
Class: lis:Stream

    
Individual: <http://example.org/5000.02.01.PU001.Pump>

    Annotations: 
        acme:visibleInDiagram "M1",
        acme:visibleInDiagram "M2",
        acme:visibleInDiagram "M3",
        dcterms:description "5000.01.01.PU001 identifies Pump 001, in plant subsection 01, in plant section 02 at Plant 5000."
    
    Types: 
        acme:E-78-130-F-M-270
    
    Facts:  
     lis:contains  acme:PU001.PumpedFluid,
     lis:hasFunctionalPart  acme:CT001.Controller,
     lis:hasFunctionalPart  acme:PU001.Housing,
     lis:hasFunctionalPart  acme:TT101.TempSensor
    
    
Individual: acme:CT001.ControlScheduler.Firmware

    Annotations: 
        acme:visibleInDiagram "M8"
    
    Types: 
        acme:InstalledSoftware
    
    Facts:  
     lis:concretizes  acme:CT001.ControlScheduler.Software,
     lis:hasFunction  acme:CT001.ControlScheduler.Function,
     lis:participantIn  acme:TT101.TempSensingActivity
    
    
Individual: acme:CT001.ControlScheduler.Function

    Annotations: 
        acme:visibleInDiagram "M8"
    
    Types: 
        acme:SoftwareAgentFunction
    
    
Individual: acme:CT001.ControlScheduler.Software

    Annotations: 
        acme:visibleInDiagram "M8"
    
    Types: 
        lis:SoftwareArtefact
    
    
Individual: acme:CT001.ControlSoftware_v1.1.1

    Annotations: 
        dcterms:description "Software installed on the pump controller CT001 to manage communication between the transmitter TT001, store the data and manage the IOT calls"
    
    Types: 
        lis:SoftwareArtefact
    
    
Individual: acme:CT001.Controller

    Annotations: 
        acme:visibleInDiagram "M3",
        dcterms:description "CT001 is the controller for Pump PU001"
    
    Types: 
        acme:ElectronicsController
    
    Facts:  
     lis:hasFunctionalPart  acme:CT001.ControlScheduler.Firmware,
     lis:hasFunctionalPart  acme:CT001.TempMonitoringFirmware,
     lis:hasFunctionalPart  acme:NotUsed.CT001.MemoryRegister001
    
    
Individual: acme:CT001.HandleTempIoTCallAndTempEstimation

    Annotations: 
        acme:visibleInDiagram "M6"
    
    Types: 
        lis:Function
    
    
Individual: acme:CT001.HandleTempIoTCallAndTempEstimation.Firmware

    Annotations: 
        acme:visibleInDiagram "M6"
    
    Types: 
        acme:InstalledSoftware
    
    Facts:  
     lis:concretizes  acme:CT001.HandleTempIoTCallAndTempEstimation.Software,
     lis:hasFunction  acme:CT001.HandleTempIoTCallAndTempEstimation,
     lis:participantIn  acme:CT001.IoTServerProcess001
    
    
Individual: acme:CT001.HandleTempIoTCallAndTempEstimation.Software

    Annotations: 
        acme:visibleInDiagram "M6"
    
    Types: 
        lis:SoftwareArtefact
    
    Facts:  
     acme:majorVersion  10,
     acme:minorVersion  2,
     acme:patchVersion  4
    
    
Individual: acme:CT001.IoTServerProcess001

    Annotations: 
        acme:visibleInDiagram "M6",
        dcterms:description "Software installed on CT001 to manage the IOT call from the client"
    
    Types: 
        acme:HandleIOTCall
    
    Facts:  
     acme:hasInput  acme:TT101.tempReading002,
     lis:hasPassiveParticipant  acme:CT101.IoT.Message,
     lis:realizes  acme:CT001.HandleTempIoTCallAndTempEstimation,
     sosa:hasResult  acme:PU001.fluidTempEst_TimeStampedIndex54678
    
    
Individual: acme:CT001.SoftwareToDIgitallyExposeTemp

    Annotations: 
        dcterms:description "Software version stored on the CT001 Firmware that is used to digitally expose (sample/ capture) the temperature on the TT101 sensor"
    
    Types: 
        acme:DigitallyExposeLiquidTemperature
    
    
Individual: acme:CT001.TempMonitoringFirmware

    Annotations: 
        dcterms:description "Firmware on CT001, the controller for Pump PU001"
    
    Types: 
        acme:InstalledSoftware
    
    Facts:  
     lis:concretizes  acme:CT001.ControlSoftware_v1.1.1,
     lis:hasFunction  acme:CT001.SoftwareToDIgitallyExposeTemp,
     lis:participantIn  acme:CT001.IoTServerProcess001
    
    
Individual: acme:CT001.temp.Result

    Annotations: 
        dcterms:description "Temperature reading of the pump housing stored in the CT001 Memory Register"
    
    Types: 
        acme:QualityDatum_2SD
    
    
Individual: acme:CT101.IoT.Message

    Annotations: 
        dcterms:description "The IoT message"
    
    Types: 
        acme:DataStream
    
    Facts:  
     lis:concretizes  acme:PU001.fluidTempEst_TimeStampedIndex54678
    
    
Individual: acme:Celsius

    Types: 
        lis:Scale
    
    
Individual: acme:NotUSed_TT101.CalibrationRange

    
Individual: acme:NotUsed.CT001.MemoryRegister001

    
Individual: acme:NotUsed_CT001.MemoryRegister002

    
Individual: acme:NotUsed_TT101.TempMonitoringSoftware_v0.0.1

    Annotations: 
        dcterms:description "Assume this software is captured in the TT101Firmware. If not then we should associate this with the temp transmitter system",
        owl:deprecated true
    
    
Individual: acme:NotUsed_TT101.TemperatureCallFunction

    
Individual: acme:NotUsed_result1

    
Individual: acme:PU001.FluidTemperature

    Annotations: 
        acme:visibleInDiagram "M1",
        dcterms:description "The actual (but not directly measured) temperature of the fluid inside PU001"
    
    Types: 
        acme:Temperature
    
    Facts:  
     lis:qualityQuantifiedAs  acme:PU001.fluidTempEst_TimeStampedIndex54678
    
    
Individual: acme:PU001.Housing

    Annotations: 
        acme:visibleInDiagram "M3",
        acme:visibleInDiagram "M4",
        dcterms:description "The housing of the pump PU001"
    
    Types: 
        acme:PumpHousing
    
    Facts:  
     lis:contains  acme:PU001.PumpedFluid,
     lis:hasPhysicalQuantity  acme:PU001.HousingTemperature
    
    
Individual: acme:PU001.HousingTemperature

    Annotations: 
        acme:visibleInDiagram "M4",
        dcterms:description "The actual temperature of the pump housing, directly measured by the temperature transmitter which is installed in a hole drilled in the pump housing"
    
    Types: 
        acme:Temperature
    
    Facts:  
     lis:qualityQuantifiedAs  acme:CT001.temp.Result
    
    
Individual: acme:PU001.PumpedFluid

    Annotations: 
        acme:visibleInDiagram "M1",
        dcterms:description "The fluid that is being pumped by the pump, it is contained by the pump housing. The fluid temperature is not measurable directly so instead the pump housing temperature is measured and an estimate of the fluid temperature made from that"
    
    Types: 
        lis:Stream
    
    Facts:  
     lis:hasPhysicalQuantity  acme:PU001.FluidTemperature
    
    
Individual: acme:PU001.fluidTempEst_TimeStampedIndex54678

    Annotations: 
        acme:visibleInDiagram "M6",
        dcterms:description "This is a time stamped value for the temperature of the fluid read in the Cloud of the user"
    
    Types: 
        acme:EstimatedDatum
    
    Facts:  
     acme:multipleOf  0.1
    
    
Individual: acme:PU001.fluidTempStoredInUsersCloud_54678

    Annotations: 
        dcterms:description "This is a time stamped value for the temperature of the fluid sent to and stored in the User's Cloud"
    
    Types: 
        acme:InstalledSoftware
    
    Facts:  
     lis:concretizes  acme:PU001.fluidTempEst_TimeStampedIndex54678
    
    
Individual: acme:TT101.DownSamplingActivity

    Annotations: 
        acme:visibleInDiagram "M5"
    
    Types: 
        lis:Activity
    
    Facts:  
     acme:hasInput  acme:TT101.tempReading001,
     sosa:hasResult  acme:TT101.tempReading002
    
    
Individual: acme:TT101.TempSensingActivity

    Annotations: 
        acme:visibleInDiagram "M4",
        acme:visibleInDiagram "M5",
        acme:visibleInDiagram "M8",
        dcterms:description "Activity involving the TT101 Temp sensor (and its functional part the Firmware) to collect temperature readings"
    
    Types: 
        acme:TemperatureSensingActivity
    
    Facts:  
     lis:hasPart  acme:TT101.DownSamplingActivity,
     lis:realizes  acme:CT001.ControlScheduler.Function
    
    
Individual: acme:TT101.TempSensor

    Annotations: 
        acme:visibleInDiagram "M3",
        acme:visibleInDiagram "M4",
        acme:visibleInDiagram "M6",
        rdfs:comment "Temperature sensor and its associated electronics (firmware) that is embedded in the pump housing"
    
    Types: 
        acme:PumpTemperatureSensor
    
    Facts:  
     lis:connectedTo  acme:PU001.Housing,
     lis:hasFunctionalPart  acme:TT101.TempSensor.Firmware,
     lis:hasQuality  acme:TT101.TempSensorCalibration
    
    
Individual: acme:TT101.TempSensor.Firmware

    Annotations: 
        dcterms:description "The version of firmware installed in PU001.TempSensor.TT101"
    
    Types: 
        acme:InstalledSoftware
    
    Facts:  
     lis:participantIn  acme:TT101.TempSensingActivity
    
    
Individual: acme:TT101.TempSensorCalibration

    Annotations: 
        acme:visibleInDiagram "M4",
        acme:visibleInDiagram "M6"
    
    Types: 
        lis:Quality
    
    
Individual: acme:TT101.tempReading001

    Annotations: 
        acme:visibleInDiagram "M5"
    
    Types: 
        lis:QualityDatum
    
    Facts:  
     acme:hasResolutionInBits  14
    
    
Individual: acme:TT101.tempReading002

    Annotations: 
        acme:visibleInDiagram "M5",
        acme:visibleInDiagram "M6"
    
    Types: 
        lis:QualityDatum
    
    Facts:  
     acme:hasResolutionInBits  8
    
    
Individual: acme:TT101Temp.Observation

    Annotations: 
        acme:visibleInDiagram "M4",
        acme:visibleInDiagram "M5",
        acme:visibleInDiagram "M6",
        dcterms:description "The activity (involving the sensor TT101) of observing the temperature"
    
    Types: 
        lis:ActivityProfile
    
    Facts:  
     lis:partOf  acme:TT101.TempSensingActivity,
     lis:profileOfQuality  acme:PU001.HousingTemperature,
     lis:profileQuantityDatum  acme:TT101.tempReading001,
     sosa:madeBySensor  acme:TT101.TempSensor,
     sosa:observedProperty  acme:PU001.HousingTemperature
    
    
Individual: acme:WotThingDescriptionLiquidTemperature-ThingDescription

    Annotations: 
        acme:visibleInDiagram "M6"
    
    Types: 
        lis:InformationObject
    
    Facts:  
     lis:concretizedBy  acme:CT001.IoTServerProcess001,
     acme:hasFormHref  "1/40000?quantity=1"
    
    
Individual: acme:softwareDeveloper_RRunner

    Annotations: 
        dcterms:description "In case we wanted to identify the software developer and use the Person class"
    
    Types: 
        lis:Person
    
    
